@prefix cc: <http://creativecommons.org/ns#> .
@prefix dc: <http://purl.org/dc/terms/> .
@prefix foaf: <http://xmlns.com/foaf/0.1/> .
@prefix oa: <http://www.w3.org/ns/oa#> .
@prefix owl: <http://www.w3.org/2002/07/owl#> .
@prefix pentandra: <https://pentandra.com/company#> .
@prefix prov: <http://www.w3.org/ns/prov#> .
@prefix rdf: <http://www.w3.org/1999/02/22-rdf-syntax-ns#> .
@prefix rdfs: <http://www.w3.org/2000/01/rdf-schema#> .
@prefix rio: <https://w3id.org/rio#> .
@prefix skos: <http://www.w3.org/2004/02/skos/core#> .
@prefix vann: <http://purl.org/vocab/vann/> .
@prefix voaf: <http://purl.org/vocommons/voaf#> .
@prefix vs: <http://www.w3.org/2003/06/sw-vocab-status/ns#> .
@prefix xsd: <http://www.w3.org/2001/XMLSchema#> .

<https://w3id.org/rio#>
  a owl:Ontology, voaf:Vocabulary ;
  dc:title "Research Intent Ontology"@en ;
  rdfs:label "Research Intent Ontology"@en ;
  dc:description """The Research Intent Ontology is a lightweight, task-oriented framework for open research utilizing the Open Web Platform. Research cases partition research into manageable units, and make explicit the chain of questions that goes through the researcher's mind as research progresses.

  Research cases are intended to be powerful enough to describe the most complex and intricate of research problems, and simple enough to be useful for informal research that could be thought of more as proactive learning. Research Cases make knowledge creation explicit and allow research and knowledge to be built upon and shared openly and in context across platforms and research disciplines."""@en ;
  rdfs:isDefinedBy rio: ;
  rdfs:seeAlso <https://pentandra.com/solutions/research-cases/>, <https://pentandra.com/solutions/research-intent-ontology/> ;
  cc:license <http://creativecommons.org/licenses/by/4.0/> ;
  cc:attributionName "Research Cases Community" ;
  cc:attributionURL <https://researchcases.org> ;
  vann:preferredNamespacePrefix "rio" ;
  vann:preferredNamespaceUri "https://w3id.org/rio#" ;
  dc:rights "Copyright © Research Cases Community" ;
  dc:creator pentandra:chris-chapman ;
  dc:contributor pentandra:katie-chapman ;
  dc:publisher pentandra:company ;
  owl:versionInfo "0.3.0" ;
  voaf:hasEquivalencesWith <http://purl.org/mp/> ;
  voaf:similar <http://purl.org/mp/> .

rio:ResearchEvent
  a owl:Class ;
  rdfs:isDefinedBy rio: ;
  rdfs:label "Research Event"@en ;
  rdfs:comment "A generic event that furthered the research process. Intended to be subclassed into more specific events."@en ;
  vs:term_status "testing" .

rio:ResearchArtifact
  a owl:Class ;
  rdfs:isDefinedBy rio: ;
  rdfs:label "Research Artifact"@en ;
  rdfs:comment "The static output of a research process."@en ;
  vs:term_status "testing" .

rio:ResearchAffordance
  a owl:Class ;
  rdfs:isDefinedBy rio: ;
  rdfs:label "Research Affordance"@en ;
  rdfs:comment "Something that affords research to be done."@en ;
  vs:term_status "testing" .

rio:ResearchPrompt
  a owl:Class ;
  rdfs:isDefinedBy rio: ;
  rdfs:label "Research Prompt"@en ;
  rdfs:comment "A research prompt, such as a question to explore or hypothesis to test."@en ;
  vs:term_status "testing" .

rio:SpecificResource
  a owl:Class ;
  rdfs:isDefinedBy rio: ;
  rdfs:subClassOf oa:ResourceSelection ;
  rdfs:label "Specific Resource"@en ;
  rdfs:comment "Instances of the SpecificResource class identify part of another resource, as used for research."@en ;
  vs:term_status "testing" .

rio:ResearchObject
  a owl:Class ;
  rdfs:isDefinedBy rio: ;
  rdfs:subClassOf rio:SpecificResource ;
  rdfs:label "Research Object"@en ;
  rdfs:comment "The object of research, i.e. whatever is being studied, searched, browsed, measured, etc. by a human or machine."@en ;
  vs:term_status "testing" .

rio:ResearchContext
  a owl:Class ;
  rdfs:isDefinedBy rio: ;
  rdfs:label "Research Context"@en ;
  rdfs:label "Контекст Дослідження"@uk ;
  rdfs:comment "A collection of research cases that are related somehow. A research context."@en ;
  vs:term_status "unstable" .
# Preliminary research needs to add sources directly to a project, because
# there may not be a question worth asking yet.

rio:ResearchCase
  a owl:Class ;
  rdfs:isDefinedBy rio: ;
  rdfs:subClassOf rio:ResearchContext ;
  rdfs:label "Research Case"@en ;
  rdfs:label "Випадок Дослідження"@uk ;
  rdfs:comment "An explicit focus on a single question, encompassing everything leading to its conclusion. Also could be thought of as an affordance to research, or an articulated intention to find an answer to a question. A fundamental unit of research."@en ;
  vs:term_status "stable" .

rio:Analysis
  a owl:Class ;
  rdfs:isDefinedBy rio: ;
  rdfs:label "Analysis"@en ;
  rdfs:label "Аналіз"@uk ;
  rdfs:comment "Some sort of presentation of the evidence. Could be a domain-specific representation."@en ;
  vs:term_status "testing" .

rio:Evidence
  a owl:Class ;
  rdfs:isDefinedBy rio: ;
  rdfs:label "Evidence"@en ;
  rdfs:label "Свідоцтво"@uk ;
  rdfs:comment "Information that could be used, in whole or in part, directly or indirectly, to answer a question, or that has bearing on the answer to a question. Evidence only exists in the context of a question."@en ;
  vs:term_status "testing" ;
  vs:moreinfo <https://pentandra.com/research/process/#evidence> .

rio:Information
  a owl:Class ;
  rdfs:isDefinedBy rio: ;
  rdfs:label "Information"@en ;
  rdfs:label "Інформація"@uk ;
  rdfs:comment "Data with context and meaning. Much of the stuff on the document web is information."@en ;
  vs:term_status "testing" ;
  vs:moreinfo <https://pentandra.com/research/process/#information> .

rio:Conclusion
  a owl:Class ;
  rdfs:isDefinedBy rio: ;
  rdfs:subClassOf rio:Information ;
  rdfs:label "Conclusion"@en ;
  rdfs:label "Висновок"@uk ;
  rdfs:comment "An answer to a research question."@en ;
  vs:term_status "testing" .

rio:Trajectory
  a owl:Class ;
  rdfs:isDefinedBy rio: ;
  rdfs:label "Trajectory"@en ;
  rdfs:label "траєкторія"@uk ;
  rdfs:comment "The trajectory is the path that the researcher moves along as research progresses. The researcher's trajectory is adjusted constantly in highly idiosyncratic ways. This term supports the intuition that all researchers have different levels of knowledge and experience, and will eventually (hopefully) converge on truth."@en ;
  vs:term_status "unstable" ;
  vs:moreinfo <http://psztajn.ced.ncsu.edu/ltbi/?page_id=1577> .

rio:Question
  a owl:Class ;
  rdfs:isDefinedBy rio: ;
  rdfs:subClassOf rio:ResearchPrompt ;
  rdfs:label "Question"@en ;
  rdfs:label "Питання"@uk ;
  rdfs:comment "A research question. Represents the direction that the researcher intends to take the research. The next thing that needs to be explored, or direction that the research needs to go."@en ;
  vs:term_status "stable" .

rio:Hypothesis
  a owl:Class ;
  rdfs:isDefinedBy rio: ;
  rdfs:subClassOf rio:ResearchPrompt ;
  rdfs:label "Hypothesis"@en ;
  rdfs:label "Гіпотеза"@uk ;
  rdfs:comment "A statement to test. A possible, though unproven, answer to a research question."@en ;
  vs:term_status "testing" .

rio:Researcher
  a owl:Class ;
  rdfs:isDefinedBy rio: ;
  rdfs:subClassOf prov:Agent ;
  rdfs:label "Researcher"@en ;
  rdfs:label "Дослідник"@uk ;
  rdfs:label "Forscher"@de ;
  rdfs:comment "A person or agent who researches"@en ;
  vs:term_status "testing" .

rio:prompt
  a owl:ObjectProperty ;
  rdfs:domain rio:ResearchCase ;
  rdfs:range rio:ResearchPrompt ;
  rdfs:isDefinedBy rio: ;
  rdfs:label "prompt"@en ;
  rdfs:label "підказка"@uk ;
  rdfs:label "Prompt"@de
  rdfs:comment "The aim of the researcher for the given research case."@en ;
  vs:term_status "stable" .

# Each research case has only one prompt.
rio:prompt a owl:FunctionalProperty .

rio:triggeredBy
  a owl:ObjectProperty ;
  rdfs:domain rio:Question ;
  rdfs:range rio:ResearchObject ;
  rdfs:isDefinedBy rio: ;
  rdfs:label "triggered by"@en ;
  rdfs:comment "Whatever prompted or triggered this question."@en ;
  vs:term_status "testing" .

rio:conclusion
  a owl:ObjectProperty ;
  rdfs:domain rio:Analysis ;
  rdfs:range rio:Conclusion ;
  rdfs:isDefinedBy rio: ;
  rdfs:label "conclusion"@en ;
  rdfs:comment "The conclusion of an analytical process that provides an answer to the question in this research case."@en ;
  vs:term_status "testing" .

rio:acceptedConclusion
  a owl:ObjectProperty ;
  rdfs:domain rio:ResearchCase ;
  rdfs:range rio:Conclusion ;
  rdfs:isDefinedBy rio: ;
  rdfs:label "accepted conclusion"@en ;
  rdfs:comment "The currently accepted conclusion to the question in this research case."@en ;
  vs:term_status "stable" .

# There is functionally one accepted conclusion per research case.
rio:acceptedConclusion a owl:FunctionalProperty .

rio:analysis
  a owl:ObjectProperty ;
  rdfs:domain rio:ResearchCase ;
  rdfs:range rio:Analysis ;
  rdfs:isDefinedBy rio: ;
  rdfs:label "analysis"@en ;
  rdfs:comment "An analysis of evidence pertinent to the question in this research case."@en ;
  vs:term_status "stable" .

rio:evidence
  a owl:ObjectProperty ;
  rdfs:domain rio:Analysis ; # Or is it a property of the research case?
  rdfs:range rio:Evidence ;
  rdfs:isDefinedBy rio: ;
  rdfs:label "evidence"@en ;
  rdfs:comment "A bit of evidence used in an analysis."@en ;
  vs:term_status "testing" .

rio:source
  a owl:ObjectProperty ;
  rdfs:domain rio:Information ;
#  rdfs:range rio:LearningContext ;
  rdfs:isDefinedBy rio: ;
  rdfs:label "source"@en ;
  rdfs:comment "The source of the information."@en ;
  vs:term_status "unstable" .

pentandra:chris-chapman
  a foaf:Person ;
  foaf:name "Chris Chapman" .

pentandra:katie-chapman
  a foaf:Person ;
  foaf:name "Katie Chapman" .

pentandra:company
  a foaf:Organization ;
  foaf:name "Pentandra Research Solutions, Inc." ;
  foaf:homepage <https://pentandra.com/> .
