@prefix cc: <http://creativecommons.org/ns#> .
@prefix owl: <http://www.w3.org/2002/07/owl#> .
@prefix prov: <http://www.w3.org/ns/prov#> .
@prefix rcases: <https://w3id.org/research/cases#> .
@prefix rdf: <http://www.w3.org/1999/02/22-rdf-syntax-ns#> .
@prefix rdfs: <http://www.w3.org/2000/01/rdf-schema#> .
@prefix skos: <http://www.w3.org/2004/02/skos/core#> .
@prefix this: <https://w3id.org/research/cases#> .
@prefix vann: <http://purl.org/vocab/vann/> .
@prefix vs: <http://www.w3.org/2003/06/sw-vocab-status/ns#> .
@prefix xsd: <http://www.w3.org/2001/XMLSchema#> .

this:
  a owl:Ontology ;
  rdfs:label "Research Cases Core Vocabulary"@en ;
  rdfs:comment """The Research Cases vocabulary is a lightweight, task-oriented framework for open research utilizing the Open Web Platform. Research cases partition research into manageable units, and make explicit the chain of questions that goes through the researcher's mind as research progresses.

  Research cases are intended to be powerful enough to describe the most complex and intricate of research problems, and simple enough to be useful for informal research that could be thought of more as proactive learning. Research Cases make knowledge creation explicit and allow research and knowledge to be built upon and shared openly and in context across platforms and research disciplines."""@en ;
  rdfs:isDefinedBy this: ;
  rdfs:seeAlso <http://researchcases.org/>, <http://pentandra.com/spec/research/research-cases/> ;
  cc:license <http://creativecommons.org/licenses/by/4.0/> ;
  cc:attributionName "Research Cases Community" ;
  cc:attributionURL <https://researchcases.org> ;
  vann:preferredNamespacePrefix "rcases" ;
  vann:preferredNamespaceUri "https://w3id.org/research/cases#" ;
  owl:versionInfo "0.3.0" .

rcases:LearningContext
  a owl:Class ;
  rdfs:isDefinedBy this: ;
  rdfs:label "Learning Context"@en ;
  rdfs:comment "Whatever is being studied, searched, browsed, measured, etc. in order for a human or machine to learn something."@en ;
  vs:term_status "stable" .

rcases:ResearchProject
  a owl:Class ;
  rdfs:isDefinedBy this: ;
  rdfs:label "Research Project"@en ;
  rdfs:label "Проект Дослідження"@uk ;
  rdfs:comment "A collection of research cases that are related somehow. A research context."@en ;
  vs:term_status "stable" .
# Preliminary research needs to add sources directly to a project, because
# there may not be a question worth asking yet.

rcases:ResearchCase
  a owl:Class ;
  rdfs:isDefinedBy this: ;
  rdfs:label "Research Case"@en ;
  rdfs:label "Випадок Дослідження"@uk ;
  rdfs:comment "An explicit focus on a single question, encompassing everything leading to its conclusion. The fundamental unit of research. Also could be thought of as an affordance to research."@en ;
  vs:term_status "stable" .

rcases:Trajectory
  a owl:Class ;
  rdfs:isDefinedBy this: ;
  rdfs:label "Trajectory"@en ;
  rdfs:label "траєкторія"@uk ;
  rdfs:comment "The trajectory is the path that the researcher takes as research progresses. The researcher's trajectory is adjusted constantly in highly idiosyncratic ways. This term supports the intuition that all researchers have different levels of knowledge and experience, and will eventually (hopefully) converge on truth."@en ;
  rdfs:seeAlso <http://psztajn.ced.ncsu.edu/ltbi/?page_id=1577> ;
  vs:term_status "testing" .

rcases:Question
  a owl:Class ;
  rdfs:isDefinedBy this: ;
  rdfs:subClassOf rcases:Trajectory ;
  rdfs:label "Question"@en ;
  rdfs:label "Питання"@uk ;
  rdfs:comment "A research question."@en ;
  vs:term_status "stable" .

rcases:Hypothesis
  a owl:Class ;
  rdfs:isDefinedBy this: ;
  rdfs:subClassOf rcases:Trajectory ;
  rdfs:label "Hypothesis"@en ;
  rdfs:label "Гіпотеза"@uk ;
  rdfs:comment "A hypothesis is a possible, though unproven, answer to a research question"@en ;
  vs:term_status "testing" .

rcases:Conclusion
  a owl:Class ;
  rdfs:isDefinedBy this: ;
  rdfs:label "Conclusion"@en ;
  rdfs:label "Висновок"@uk ;
  rdfs:comment "An answer to a research question."@en ;
  vs:term_status "stable" .

rcases:Researcher
  a owl:Class ;
  rdfs:isDefinedBy this: ;
  rdfs:subClassOf prov:Agent ;
  rdfs:label "Researcher"@en ;
  rdfs:label "Дослідник"@uk ;
  rdfs:comment "A person who researches"@en ;
  vs:term_status "testing" .

rcases:purpose
  a owl:DatatypeProperty ;
  rdfs:domain rcases:ResearchProject ;
  rdfs:isDefinedBy this: ;
  rdfs:label "purpose"@en ;
  rdfs:label "мета"@uk ;
  rdfs:comment "The purpose for engaging in the research project. Could be a general statement of the problem being investigated."@en ;
  vs:term_status "testing" .

rcases:question
  a owl:ObjectProperty ;
  rdfs:domain rcases:ResearchCase ;
  rdfs:range rcases:Question ;
  rdfs:isDefinedBy this: ;
  rdfs:label "question"@en ;
  rdfs:label "питання"@uk ;
  rdfs:comment "A focused research question."@en ;
  vs:term_status "stable" .

# There is functionally one question per research case.
rcases:question a owl:FunctionalProperty .

rcases:trigger
  a owl:ObjectProperty ;
  rdfs:domain rcases:ResearchCase ;
  rdfs:range rcases:LearningContext ;
  rdfs:isDefinedBy this: ;
  rdfs:label "trigger"@en ;
  rdfs:comment "The learning context, if any, that triggered the creation of this research context"@en ;
  vs:term_status "testing" .
