@prefix cc: <http://creativecommons.org/ns#> .
@prefix owl: <http://www.w3.org/2002/07/owl#> .
@prefix prov: <http://www.w3.org/ns/prov#> .
@prefix rcases: <https://w3id.org/research/cases#> .
@prefix rdf: <http://www.w3.org/1999/02/22-rdf-syntax-ns#> .
@prefix rdfs: <http://www.w3.org/2000/01/rdf-schema#> .
@prefix skos: <http://www.w3.org/2004/02/skos/core#> .
@prefix vann: <http://purl.org/vocab/vann/> .
@prefix vs: <http://www.w3.org/2003/06/sw-vocab-status/ns#> .
@prefix xsd: <http://www.w3.org/2001/XMLSchema#> .

<https://w3id.org/research/cases#>
  a owl:Ontology ;
  rdfs:label "Research Cases Core Vocabulary"@en ;
  rdfs:comment """The Research Cases vocabulary is a lightweight, task-oriented framework for open research utilizing the Open Web Platform. Research cases partition research into manageable units, and make explicit the chain of questions that goes through the researcher's mind as research progresses.

  Research cases are intended to be powerful enough to describe the most complex and intricate of research problems, and simple enough to be useful for informal research that could be thought of more as proactive learning. Research Cases make knowledge creation explicit and allow research and knowledge to be built upon and shared openly and in context across platforms and research disciplines."""@en ;
  rdfs:isDefinedBy rcases: ;
  rdfs:seeAlso <http://researchcases.org/>, <http://pentandra.com/spec/research/research-cases/> ;
  cc:license <http://creativecommons.org/licenses/by/4.0/> ;
  cc:attributionName "Research Cases Community" ;
  cc:attributionURL <https://researchcases.org> ;
  vann:preferredNamespacePrefix "rcases" ;
  vann:preferredNamespaceUri "https://w3id.org/research/cases#" ;
  owl:versionInfo "0.3.0" .

rcases:LearningContext
  a owl:Class ;
  rdfs:isDefinedBy rcases: ;
  rdfs:label "Learning Context"@en ;
  rdfs:comment "Whatever is being studied, searched, browsed, measured, etc. in order for a human or machine to learn something."@en ;
  vs:term_status "stable" .

rcases:ResearchContext
  a owl:Class ;
  rdfs:isDefinedBy rcases: ;
  rdfs:label "Research Context"@en ;
  rdfs:label "Контекст Дослідження"@uk ;
  rdfs:comment "A collection of research cases that are related somehow. A research context."@en ;
  vs:term_status "unstable" .
# Preliminary research needs to add sources directly to a project, because
# there may not be a question worth asking yet.

rcases:ResearchCase
  a owl:Class ;
  rdfs:isDefinedBy rcases: ;
  rdfs:subClassOf prov:Plan ;
  rdfs:label "Research Case"@en ;
  rdfs:label "Випадок Дослідження"@uk ;
  rdfs:comment "An explicit focus on a single question, encompassing everything leading to its conclusion. Also could be thought of as an affordance to research, or an articulated intention to find an answer to a question. The fundamental unit of research."@en ;
  vs:term_status "stable" .

rcases:Analysis
  a owl:Class ;
  rdfs:isDefinedBy rcases: ;
  rdfs:label "Analysis"@en ;
  rdfs:label "Аналіз"@uk ;
  rdfs:comment "Some sort of presentation of the evidence. Could be a domain-specific representation."@en ;
  vs:term_status "testing" .

rcases:Evidence
  a owl:Class ;
  rdfs:isDefinedBy rcases: ;
  rdfs:label "Evidence"@en ;
  rdfs:label "Свідоцтво"@uk ;
  rdfs:comment "Information that could be used, in whole or in part, directly or indirectly, to answer a question, or that has bearing on the answer to a question. Evidence only exists in the context of a question."@en ;
  vs:term_status "testing" ;
  vs:moreinfo <http://pentandra.com/research/process/#dfn:evidence> .

rcases:Information
  a owl:Class ;
  rdfs:isDefinedBy rcases: ;
  rdfs:label "Information"@en ;
  rdfs:label "Інформація"@uk ;
  rdfs:comment "Data with context and meaning. Much of the stuff on the document web is information."@en ;
  vs:term_status "testing" ;
  vs:moreinfo <http://pentandra.com/research/process/#dfn:information> .

rcases:Conclusion
  a owl:Class ;
  rdfs:isDefinedBy rcases: ;
  rdfs:subClassOf rcases:Information ;
  rdfs:label "Conclusion"@en ;
  rdfs:label "Висновок"@uk ;
  rdfs:comment "An answer to a research question."@en ;
  vs:term_status "testing" .

rcases:Intention
  a owl:Class ;
  rdfs:isDefinedBy rcases: ;
  rdfs:label "Intention"@en ;
  rdfs:label "Намір"@uk ;
  rdfs:comment "The next step that the researcher intends to take in the research process. The next thing that needs to be explored, or direction the research needs to go."@en ;
  vs:term_status "testing" .

rcases:Trajectory
  a owl:Class ;
  rdfs:isDefinedBy rcases: ;
  rdfs:label "Trajectory"@en ;
  rdfs:label "траєкторія"@uk ;
  rdfs:comment "The trajectory is the path that the researcher takes as research progresses. The researcher's trajectory is adjusted constantly in highly idiosyncratic ways. This term supports the intuition that all researchers have different levels of knowledge and experience, and will eventually (hopefully) converge on truth."@en ;
  vs:term_status "unstable" ;
  vs:moreinfo <http://psztajn.ced.ncsu.edu/ltbi/?page_id=1577> .

rcases:Question
  a owl:Class ;
  rdfs:isDefinedBy rcases: ;
  rdfs:subClassOf rcases:Intention ;
  rdfs:label "Question"@en ;
  rdfs:label "Питання"@uk ;
  rdfs:comment "A research question."@en ;
  vs:term_status "stable" .

rcases:Hypothesis
  a owl:Class ;
  rdfs:isDefinedBy rcases: ;
  rdfs:subClassOf rcases:Intention ;
  rdfs:label "Hypothesis"@en ;
  rdfs:label "Гіпотеза"@uk ;
  rdfs:comment "A hypothesis is a possible, though unproven, answer to a research question"@en ;
  vs:term_status "testing" .

rcases:Researcher
  a owl:Class ;
  rdfs:isDefinedBy rcases: ;
  rdfs:subClassOf prov:Agent ;
  rdfs:label "Researcher"@en ;
  rdfs:label "Дослідник"@uk ;
  rdfs:comment "A person who researches"@en ;
  vs:term_status "testing" .

rcases:intent
  a owl:ObjectProperty ;
  rdfs:domain rcases:ResearchCase ;
  rdfs:range rcases:Intention ;
  rdfs:isDefinedBy rcases: ;
  rdfs:label "intent"@en ;
  rdfs:label "Замір"@uk ;
  rdfs:comment "What the researcher is intending to do next. The next step the researcher is taking."@en ;
  vs:term_status "stable" .

# There is functionally one question per research case.
rcases:question a owl:FunctionalProperty .

rcases:triggeredBy
  a owl:ObjectProperty ;
  rdfs:domain rcases:Question ;
  rdfs:range rcases:LearningContext ;
  rdfs:isDefinedBy rcases: ;
  rdfs:label "triggered by"@en ;
  rdfs:comment "The learning context, if any, that prompted or triggered this question."@en ;
  vs:term_status "testing" .

rcases:conclusion
  a owl:ObjectProperty ;
  rdfs:domain rcases:Analysis ;
  rdfs:range rcases:Conclusion ;
  rdfs:isDefinedBy rcases: ;
  rdfs:label "conclusion"@en ;
  rdfs:comment "An answer to the question"@en ;
  vs:term_status "testing" .

rcases:acceptedConclusion
  a owl:ObjectProperty ;
  rdfs:domain rcases:ResearchCase ;
  rdfs:range rcases:Conclusion ;
  rdfs:isDefinedBy rcases: ;
  rdfs:label "accepted conclusion"@en ;
  rdfs:comment "The currently accepted conclusion to the question in this research case"@en ;
  vs:term_status "stable" .

# There is functionally one accepted conclusion per research case.
rcases:acceptedConclusion a owl:FunctionalProperty .

rcases:analysis
  a owl:ObjectProperty ;
  rdfs:domain rcases:ResearchCase ;
  rdfs:range rcases:Analysis ;
  rdfs:isDefinedBy rcases: ;
  rdfs:label "analysis"@en ;
  rdfs:comment "An analysis of evidence pertinent to the question in this research case"@en ;
  vs:term_status "stable" .

rcases:evidence
  a owl:ObjectProperty ;
  rdfs:domain rcases:Analysis ; # Or is it a property of the research case?
  rdfs:range rcases:Evidence ;
  rdfs:isDefinedBy rcases: ;
  rdfs:label "evidence"@en ;
  rdfs:comment "Evidence used in an analysis"@en ;
  vs:term_status "testing" .
